Cheriot/SpecIsolation.v
@@ -3,65 +3,65 @@ Require Import ProcKami.Cheriot.Lib ProcKami.Cheriot.Types ProcKami.Cheriot.Core
 
 Section InBoundsTy.
   Variable ty: Kind -> Type.
-  Variable x : Bit 32 @# ty.
-  Variable inCap: Cap @# ty.
-  Variable inVal: Bit 32 @# ty.
+  Variable x : Addr @# ty.
+  Variable cap: FullCapWithTag @# ty.
 
   Local Open Scope kami_expr.
 
-  Let inRange := getCapBaseTop (STRUCT { "cap" ::= inCap; "val" ::= inVal }).
-
   Definition inBounds :=
-    ( LETE inRangeVal <- inRange;
-      RetE ((x >= #inRangeVal @% "base") && (ZeroExtend 1 x < #inRangeVal @% "top"))).
+    ( LETE inRangeVal <- getCapBaseTop (rmTag cap);
+      RetE (cap @% "tag" && (x >= #inRangeVal @% "base") && (ZeroExtend 1 x < #inRangeVal @% "top"))).
 
   Definition systemAccess :=
-    ( LETC perms <- getCapPerms inCap;
-      RetE (#perms @% "SR") ).
+    ( LETC perms <- getCapPerms (cap @% "cap");
+      RetE (cap @% "tag" && #perms @% "SR") ).
 End InBoundsTy.
 
 Section InBoundsInits.
-  Variable x: word 32.
-  Variable rfInit: Fin.t 32 -> type FullCapWithTag.
-  Variable capPcInit: type Cap.
-  Variable valPcInit: word 32.
+  Variable x: word AddrSz.
+  Variable rfInit: Fin.t NumRegs -> type FullCapWithTag.
+  Variable pccInit: type FullCapWithTag.
 
   Local Open Scope kami_expr.
 
   Definition InBoundsRf :=
-    exists i, evalLetExpr (inBounds (Const _ x)
-                             (Var type (SyntaxKind _) (rfInit i) @% "cap")
-                             (Var type (SyntaxKind _) (rfInit i) @% "val")) = true.
+    exists i, evalLetExpr (inBounds (Const _ x) (Const _ (convTypeToConst (rfInit i)))) = true.
+
   Definition InBoundsPc :=
-    evalLetExpr (inBounds (Const _ x) (Const _ (convTypeToConst capPcInit)) (Const _ valPcInit)) = true.
+    evalLetExpr (inBounds (Const _ x) (Const _ (convTypeToConst pccInit))) = true.
 
   Definition SystemAccessRf :=
-    exists i, evalLetExpr (systemAccess (Var type (SyntaxKind _) (rfInit i) @% "cap")) = true.
+    exists i, evalLetExpr (systemAccess (Const _ (convTypeToConst (rfInit i)))) = true.
 
   Definition SystemAccessPc :=
-    evalLetExpr (systemAccess (Const _ (convTypeToConst capPcInit))) = true.
+    evalLetExpr (systemAccess (Const _ (convTypeToConst pccInit))) = true.
 End InBoundsInits.
 
 Section InBoundsCoreConfig.
-  Variable x: word 32.
+  Variable x: word AddrSz.
   Variable p: CoreConfigParams.
-  Definition InBoundsInit := InBoundsRf x (@regsInit p) \/ InBoundsPc x (@pcCapInit p)
-                                                             (wcombine (@pcValInit p) (wzero 2)).
-  Definition SystemAccessInit := SystemAccessRf (@regsInit p) \/ SystemAccessPc (@pcCapInit p).
+
+  Let pccInit := evalExpr (STRUCT {"tag" ::= Const _ true ;
+                                    "cap" ::= Const _ (convTypeToConst (@pcCapInit p)) ;
+                                    "val" ::= Const _ (wcombine (@pcValInit p) (wzero 2)) })%kami_expr.
+  
+  Definition InBounds := InBoundsRf x (@regsInit p) \/ InBoundsPc x pccInit.
+
+  Definition SystemAccess := SystemAccessRf (@regsInit p) \/ SystemAccessPc pccInit.
 End InBoundsCoreConfig.
 
 Record SpecIsolation := {
     cores: list CoreConfigParams;
     disjointNamesCores: NoDup (map (@procName) cores);
-    disjointBoundsCores: forall x p, In p cores -> InBoundsInit x p -> forall q,
-                                         In q cores -> InBoundsInit x q -> @procName p <> @procName q -> False;
-    noScrAccessCores: forall p, In p cores -> SystemAccessInit p -> False;
+    disjointBoundsCores: forall x p, In p cores -> InBounds x p -> forall q,
+                                         In q cores -> InBounds x q -> @procName p = @procName q;
+    noScrAccessCores: forall p, In p cores -> SystemAccess p -> False;
     noTrapCores: forall p, In p cores -> @hasTrap p = false;
     trapCore: CoreConfigParams;
     trapCoreMemSize: forall p, In p cores -> @LgNumMemBytes (@memParams p) = @LgNumMemBytes (@memParams trapCore);
-    disjointTrapCore: forall x p, In p cores -> InBoundsInit x p -> InBoundsInit x trapCore -> False;
+    disjointTrapCore: forall x p, In p cores -> InBounds x p -> InBounds x trapCore -> False;
     sameMemTrapCore: forall x p,
-      In p cores -> InBoundsInit x p ->
+      In p cores -> InBounds x p ->
       evalExpr (Var type (SyntaxKind (Array _ (Bit 8))) (@memInit (@memParams trapCore)) @[Const _ x])%kami_expr =
         evalExpr (Var type (SyntaxKind (Array _ (Bit 8)))(@memInit (@memParams p)) @[Const _ x])%kami_expr;
     trapCoreHasTrap: @hasTrap trapCore = true;
