Cheriot/SpecRun.v
@@ -19,77 +19,160 @@ Section Run.
 
   Local Notation "@^ x" := (procName ++ "_" ++ x)%string (at level 0).
 
-  (* TODO: Fix rules to make them disjoint; example setPcException is always called even if there's no exception in specInstBoundsException and specInstIllegalException. TODO *)
-  Definition setTrapException (pred isCap isScr: Bool @# ty) (idx: Bit RegFixedIdSz @# ty)
-    (cause value: Data @# ty):
-    ActionT ty Void :=
-    ( Read pcCap : Cap <- @^pcCapReg;
-      Read pcVal : Addr <- @^pcValReg;
-      WriteIf pred Then @^mepccReg : FullCapWithTag <- STRUCT { "tag" ::= $$true;
-                                                                "cap" ::= #pcCap;
-                                                                "val" ::= #pcVal };
-      WriteIf pred Then @^mCauseReg : Data <- ITE isCap $CapException cause;
-      WriteIf pred Then @^mtValReg : Data <-
-                                       ITE isCap
+  Definition handleException
+    (pred isException baseException scrException pcCapException wbScr wbCsr changePcVal changePcCap: Bool @# ty)
+    (newPcVal: Addr @# ty) (newPcCap: Cap @# ty) (newScr: FullCapWithTag @# ty) (newCsr: Data @# ty)
+    (scrIdx: ScrId @# ty) (csrIdx: Bit CsrIdSz @# ty) (exceptionCause exceptionVal: Data @# ty)
+    (exceptionIdx: Bit RegFixedIdSz @# ty) : ActionT ty Void :=
+    ( Read pcVal : Addr <- @^pcValReg;
+      Read pcCap : Cap <- @^pcCapReg;
+      LET pcc : FullCapWithTag <- STRUCT { "tag" ::= $$true;
+                                           "cap" ::= #pcCap;
+                                           "val" ::= #pcVal };
+      LETA exceptionPc <- if hasTrap
+                          then
+                            ( Read mtcc : FullCapWithTag <- @^mtccReg;
+                              Ret #mtcc )
+                          else Ret #pcc ;
+
+      WriteIf pred Then
+        @^pcValReg : Addr <- (IF isException
+                              then #exceptionPc @% "val"
+                              else ITE changePcVal newPcVal #pcVal);
+      WriteIf pred Then
+        @^pcCapReg : Cap <- (IF isException
+                             then #exceptionPc @% "cap"
+                             else ITE changePcCap newPcCap #pcCap);
+
+      if hasTrap
+      then
+        ( Read mepccVal : FullCapWithTag <- @^mepccReg;
+          WriteIf pred Then
+            @^mepccReg : FullCapWithTag <- (IF isException
+                                            then #pcc
+                                            else (IF scrIdx == $$(getRegScrId mepcc)
+                                                  then newScr
+                                                  else #mepccVal));
+
+          Read mStatusVal : Data <- @^mStatusReg;
+          LET mStatusArr <- unpack (Array Xlen Bool) #mStatusVal;
+          LET newMStatusVal <- pack (UpdateArrayConst (UpdateArrayConst #mStatusArr (@natToFin 3 _) ($$false))
+                                       (@natToFin 7 _) (#mStatusArr ![3]));
+          WriteIf pred Then
+            @^mStatusReg : Data <- (IF isException
+                                    then #newMStatusVal
+                                    else (IF csrIdx == $$(getCsrId mstatus)
+                                          then newCsr
+                                          else #mStatusVal));
+
+          Read mCauseVal : Data <- @^mCauseReg;
+          WriteIf pred Then
+            @^mCauseReg : Data <- (IF isException
+                                   then ITE baseException exceptionCause $CapException
+                                   else (IF wbScr && csrIdx == $$(getCsrId mcause)
+                                         then newCsr
+                                         else #mCauseVal));
+          
+          Read mtValVal : Data <- @^mtValReg;
+          WriteIf pred Then
+            @^mtValReg : Data <- (IF isException
+                                  then ITE baseException
+                                         exceptionVal
                                          (ZeroExtendTruncLsb Xlen
-                                            (pack (STRUCT { "S" ::= isScr;
-                                                            "capIdx" ::= idx;
-                                                            "cause" ::= ZeroExtendTruncLsb RegFixedIdSz cause })))
-                                         value;
-      Retv ).
+                                            (pack (STRUCT { "S" ::= scrException;
+                                                            "capIdx" ::= exceptionIdx;
+                                                            "cause" ::= ZeroExtendTruncLsb RegFixedIdSz
+                                                                          exceptionCause })))
+                                  else (IF wbCsr && csrIdx == $$(getCsrId mtval)
+                                        then newCsr
+                                        else #mtValVal));
+          
+          
+          LETA _ <- writeRegsPred procName scrRegInfos
+                      (pred && !isException && wbScr && (scrIdx != $$(getRegScrId mepcc)))
+                      scrIdx newScr;
 
-  Definition setException (pred isCap isScr: Bool @# ty) (idx: Bit RegFixedIdSz @# ty)
-    (cause value: Data @# ty) :=
-    if hasTrap
-    then setTrapException pred isCap isScr idx cause value
-    else Retv.
+          LETA _ <- writeRegsPred procName csrRegInfos
+                      (pred && !isException && wbCsr &&
+                         (csrIdx != $$(getCsrId mstatus)) &&
+                         (csrIdx != $$(getCsrId mcause)) &&
+                         (csrIdx != $$(getCsrId mtval)))
+                      csrIdx newCsr;
 
-  Definition gotoMtcc (pred: Bool @# ty) :=
-    if hasTrap
-    then (
-        Read mtcc : FullCapWithTag <- @^mtccReg;
-        WriteIf pred Then @^pcCapReg : Cap <- #mtcc @% "cap";
-        WriteIf pred Then @^pcValReg : Addr <- #mtcc @% "val";
+          Retv
+        )
+      else Retv).
+
+  Definition specTimerIncAndInterruptSetRule :=
+    ( if hasTrap
+      then
+      ( Read mTime : Data <- @^mTimeReg;
+        Read mTimeCmp: Data <- @^mTimeCmpReg;
+        LET msb <- UniBit (TruncMsb (Xlen - 1) 1) (#mTime - #mTimeCmp);
+        WriteIf (isZero #msb) Then @^mtiReg : Bool <- $$true;
+        Write @^mTimeReg : Data <- #mTime + $1;
         Retv )
-    else Retv.
-  
-  Definition specInstBoundsException :=
-    ( Read pcCap : Cap <- @^pcCapReg;
-      Read pcVal : Addr <- @^pcValReg;
-      LETAE baseTop <- getCapBaseTop (STRUCT { "cap" ::= #pcCap; "val" ::= #pcVal });
-      LET topBound <- ZeroExtend 1 #pcVal + $4 <= (#baseTop @% "top");
-      LETA _ <- gotoMtcc (!#topBound);
-      setException (!#topBound) ($$true) ($$false) $0 ($CapBoundsViolation) $0).
+      else Retv ).
 
-  Definition specInstIllegalException (ies: list (InstEntry FullOutput)) :=
+  Definition specTimerInterruptTakeRule :=
+    ( if hasTrap
+      then
+        ( Read mti : Bool <- @^mtiReg;
+          Write @^mtiReg : Bool <- $$false;
+          handleException ($$true) #mti ($$true) ($$false) ($$false) ($$false) ($$false) ($$false) ($$false)
+            ($0) ($$(getDefaultConst Cap)) ($$(getDefaultConst FullCapWithTag)) ($0)
+            ($0) ($0) ({<$$WO~1, $$(natToWord (Xlen-1) TimerInterrupt)>}) ($0)
+            ($0) )
+      else Retv ).
+  
+  Definition specInstBoundsExceptionRule :=
     ( Read pcCap : Cap <- @^pcCapReg;
       Read pcVal : Addr <- @^pcValReg;
       LETAE baseTop <- getCapBaseTop (STRUCT { "cap" ::= #pcCap; "val" ::= #pcVal });
-      LET topBound <- ZeroExtend 1 #pcVal + $4 <= (#baseTop @% "top");
+      LET topBound <- ZeroExtend 1 #pcVal + $(InstSz/8) <= (#baseTop @% "top");
+      if hasTrap
+      then
+        ( Read mti : Bool <- @^mtiReg;
+          handleException (!#mti) (!#topBound) ($$false) ($$false) ($$true) ($$false) ($$false) ($$false) ($$false)
+            ($0) ($$(getDefaultConst Cap)) ($$(getDefaultConst FullCapWithTag)) ($0)
+            ($0) ($0) ($CapBoundsViolation) ($0)
+            ($0) )
+      else Retv ).
+
+  Definition specInstIllegalExceptionRule (ies: list InstEntrySpec) :=
+    ( Read pcCap : Cap <- @^pcCapReg;
+      Read pcVal : Addr <- @^pcValReg;
+      LETAE baseTop <- getCapBaseTop (STRUCT { "cap" ::= #pcCap; "val" ::= #pcVal });
+      LET topBound <- ZeroExtend 1 #pcVal + $(InstSz/8) <= (#baseTop @% "top");
       Read memArr : Array (NumMemBytes * NumBanks) (Bit 8) <- memArray;
       LET inst <- pack (readArrayConstSize #pcVal #memArr (InstSz/8));
       Read regs : Array NumRegs FullCapWithTag <- regsArray;
       LET illegal <- CABool And (map (fun ie => !(matchUniqId #inst (uniqId ie))) ies);
-      LETA _ <- gotoMtcc (#topBound && #illegal);
-      setException (#topBound && #illegal) $$false $$false
-        $0 $InstIllegal (ZeroExtendTruncLsb Xlen #inst)).
+      if hasTrap
+      then
+        ( Read mti : Bool <- @^mtiReg;
+          handleException (!#mti && #topBound) #illegal ($$true) ($$false) ($$true) ($$false) ($$false) ($$false) ($$false)
+            ($0) ($$(getDefaultConst Cap)) ($$(getDefaultConst FullCapWithTag)) ($0)
+            ($0) ($0) ($InstIllegal) (ZeroExtendTruncLsb Xlen #inst)
+            ($0) )
+      else Retv ).
   
   Definition specDecExecRule (ie: InstEntrySpec) :=
     ( Read pcCap : Cap <- @^pcCapReg;
       Read pcVal : Addr <- @^pcValReg;
       LETAE baseTop <- getCapBaseTop (STRUCT { "cap" ::= #pcCap; "val" ::= #pcVal });
-      LET topBound <- ZeroExtend 1 #pcVal + $4 <= (#baseTop @% "top");
+      LET topBound <- ZeroExtend 1 #pcVal + $(InstSz/8) <= (#baseTop @% "top");
       Read memArr : Array (NumMemBytes * NumBanks) (Bit 8) <- memArray;
       LET inst <- pack (readArrayConstSize #pcVal #memArr (InstSz/8));
       Read regs : Array NumRegs FullCapWithTag <- regsArray;
       let instProps := instProperties ie in
       LET cs1Idx <- if (weq (implicitReg instProps) (wzero _)) then (rs1 #inst) else $$(implicitReg instProps);
-      LET cs2Idx <- rs2 #inst;
+      LET cs2Idx <- rs2Fixed #inst;
       LET scrIdx <- if (weq (implicitScr instProps) (wzero _))
                     then (rs2Fixed #inst) else $$(implicitScr instProps);
       LET csrIdx <- if (weq (implicitCsr instProps) (wzero _)) then (imm #inst) else $$(implicitCsr instProps);
       LET cs1 <- #regs@[#cs1Idx];
-      LET cs2 <- #regs@[#cs2Idx];
+      LET cs2 <- #regs@[ZeroExtendTruncLsb RegIdSz #cs2Idx];
       LETA scr <- readRegs procName scrRegInfos #scrIdx FullCapWithTag;
       LETA csr <- readRegs procName csrRegInfos #csrIdx Data;
       LETAE out <- spec ie (STRUCT { "cap" ::= #pcCap; "val" ::= #pcVal }) #inst #cs1 #cs2 #scr #csr;
@@ -106,30 +189,17 @@ Section Run.
       LET instMatch <- matchUniqId #inst (uniqId ie);
       LET updRegs <- #regs @[ #cdIdx <- ITE ((#cdIdx != $0) && (#out @% "wb?")) #cd (#regs@[#cdIdx])];
 
-      LET matchNoException <- #topBound && #instMatch && !(#out @% "exception?");
-
-      WriteIf #matchNoException Then
-        regsArray: Array NumRegs FullCapWithTag <- #updRegs;
-      LETA _ <- storeReqSpec procName (#matchNoException && (#out @% "mem?") && (#out @% "store?")) (#out @% "pcMemAddr")
-                  (#out @% "memSize") (#out @% "memCap?")
-                  (STRUCT { "tag" ::= #out @% "cdTag";
-                            "cap" ::= #out @% "cdCap";
-                            "val" ::= #out @% "cdVal" });
-
-      Read mtcc : FullCapWithTag <- @^mtccReg;
-      WriteIf (#topBound && #instMatch) Then
-        @^pcCapReg : Cap <- (IF (#out @% "exception?")
-                             then #mtcc @% "cap"
-                             else ITE (#out @% "changePcCap?") (#out @% "pcCap") #pcCap);
-      WriteIf (#topBound && #instMatch) Then
-        @^pcValReg : Addr <- (IF (#out @% "exception?")
-                              then #mtcc @% "val"
-                              else ITE (#out @% "taken?") (#out @% "pcMemAddr") (#pcVal + $(InstSz/8)));
-
-      LET matchException <- #topBound && #instMatch && (#out @% "exception?");
-
-      setException #matchException (!(#out @% "baseException?")) (#out @% "scrException?")
-        (ITE (#out @% "pcCapException?") $0 (ZeroExtendTruncLsb RegFixedIdSz #cs1Idx))
-        (#out @% "exceptionCause") (#out @% "exceptionValue")
-      ).
+      LETA mti <- if hasTrap
+                  then ( Read mti : Bool <- @^mtiReg;
+                         Ret #mti )
+                  else Ret $$false;
+      handleException (!#mti && #topBound && #instMatch) (!(#out @% "exception?")) (#out @% "baseException?")
+        (#out @% "scrException?") (#out @% "pcCapException?") (#out @% "wbScr?") (#out @% "wbCsr?")
+        ($$true) (#out @% "changePcCap?")
+        (ITE (#out @% "taken?") (#out @% "pcMemAddr") (#pcVal + $(InstSz/8))) (#out @% "pcCap")
+        (STRUCT { "tag" ::= #out @% "scrTag";
+                  "cap" ::= #out @% "scrCap";
+                  "val" ::= #out @% "scrVal" }) (#out @% "csrVal")
+        #cs2Idx #csrIdx (#out @% "exceptionCause") (#out @% "exceptionValue")
+        (ITE (#out @% "pcCapException?") $0 (ZeroExtendTruncLsb RegFixedIdSz #cs1Idx)) ).
 End Run.
